case_studies/Infinitary_Lambda_Calculus/ILC2.thy
@@ -2,9 +2,9 @@ theory ILC2
 imports ILC "Case_Studies.Generic_Barendregt_Enhanced_Rule_Induction"
 begin
 
-instance ivar :: uncountable_regular ..
+instance ivar :: covar ..
 
-lemma small_image_sset[simp,intro]: "inj_on (f :: 'a \<Rightarrow> 'a :: {uncountable_regular}) (dsset xs) \<Longrightarrow> small (f ` dsset xs)"
+lemma small_image_sset[simp,intro]: "inj_on (f :: 'a \<Rightarrow> 'a :: {covar}) (dsset xs) \<Longrightarrow> small (f ` dsset xs)"
   by (auto simp: small_def dsset_card_ls simp flip: dsset_dsmap)
 
 lemma snth_equiv[equiv]:
